<http://vcell.org/sbpax3#SBVocabulary> <http://www.w3.org/2000/01/rdf-schema#comment> "Controlled vocabulary that describes a systems biology concept, such as a Systems Biology Ontology term.\nExamples: an SBO term; an SBML element name"^^<http://www.w3.org/2001/XMLSchema#string> .
<http://vcell.org/sbpax3#SBVocabulary> <http://www.w3.org/2000/01/rdf-schema#subClassOf> <http://www.biopax.org/release/biopax-level3.owl#ControlledVocabulary> .
<http://vcell.org/sbpax3#SBVocabulary> <http://www.w3.org/1999/02/22-rdf-syntax-ns#type> <http://www.w3.org/2002/07/owl#Class> .
<http://vcell.org/sbpax3#SBMeasurable> <http://www.w3.org/2000/01/rdf-schema#comment> "An entity that can be characterized by one or more systems biology terms and that can be represented by a number and a unit.\nExample: a parameter in a particular instance."^^<http://www.w3.org/2001/XMLSchema#string> .
<http://vcell.org/sbpax3#SBMeasurable> <http://www.w3.org/2000/01/rdf-schema#subClassOf> <http://vcell.org/sbpax3#SBEntity> .
<http://vcell.org/sbpax3#SBMeasurable> <http://www.w3.org/1999/02/22-rdf-syntax-ns#type> <http://www.w3.org/2002/07/owl#Class> .
<http://vcell.org/sbpax3#sbSubEntity> <http://www.w3.org/2000/01/rdf-schema#comment> "A systems biology entity that is a part, attribute or subset of this systems biology entity.\nExamples: rate law of an interaction; parameters of a rate law."^^<http://www.w3.org/2001/XMLSchema#string> .
<http://vcell.org/sbpax3#sbSubEntity> <http://www.w3.org/2000/01/rdf-schema#range> <http://vcell.org/sbpax3#SBEntity> .
<http://vcell.org/sbpax3#sbSubEntity> <http://www.w3.org/2000/01/rdf-schema#domain> <http://vcell.org/sbpax3#SBEntity> .
<http://vcell.org/sbpax3#sbSubEntity> <http://www.w3.org/1999/02/22-rdf-syntax-ns#type> <http://www.w3.org/2002/07/owl#ObjectProperty> .
<http://vcell.org/sbpax3#SBEntity> <http://www.w3.org/2000/01/rdf-schema#comment> "An entity that can be characterized by one or more systems biology terms.\nExamples: a BioPAX entity; a rate law or a parameter in a particular instance."^^<http://www.w3.org/2001/XMLSchema#string> .
<http://vcell.org/sbpax3#SBEntity> <http://www.w3.org/1999/02/22-rdf-syntax-ns#type> <http://www.w3.org/2002/07/owl#Class> .
<http://vcell.org/sbpax3> <http://www.w3.org/2002/07/owl#imports> <http://vcell.org/uome/expressions/> .
<http://vcell.org/sbpax3> <http://www.w3.org/2002/07/owl#imports> <http://www.biopax.org/release/biopax-level3.owl> .
<http://vcell.org/sbpax3> <http://www.w3.org/1999/02/22-rdf-syntax-ns#type> <http://www.w3.org/2002/07/owl#Ontology> .
<http://vcell.org/sbpax3#hasNumber> <http://www.w3.org/2000/01/rdf-schema#comment> "The number representing this measurable systems biology entity.\nExample: a concentration of 5 mol/l would have the number 5 together with the unit string \"mol/l\""^^<http://www.w3.org/2001/XMLSchema#string> .
<http://vcell.org/sbpax3#hasNumber> <http://www.w3.org/2000/01/rdf-schema#range> <http://www.w3.org/2001/XMLSchema#float> .
<http://vcell.org/sbpax3#hasNumber> <http://www.w3.org/2000/01/rdf-schema#domain> <http://vcell.org/sbpax3#SBEntity> .
<http://vcell.org/sbpax3#hasNumber> <http://www.w3.org/1999/02/22-rdf-syntax-ns#type> <http://www.w3.org/2002/07/owl#DatatypeProperty> .
<http://vcell.org/sbpax3#sbTerm> <http://www.w3.org/2000/01/rdf-schema#comment> "The systems biology term that this entity is an instance of.\nExamples: an SBO term; an SBML element name."^^<http://www.w3.org/2001/XMLSchema#string> .
<http://vcell.org/sbpax3#sbTerm> <http://www.w3.org/2000/01/rdf-schema#range> <http://vcell.org/sbpax3#SBVocabulary> .
<http://vcell.org/sbpax3#sbTerm> <http://www.w3.org/2000/01/rdf-schema#domain> <http://vcell.org/sbpax3#SBEntity> .
<http://vcell.org/sbpax3#sbTerm> <http://www.w3.org/1999/02/22-rdf-syntax-ns#type> <http://www.w3.org/2002/07/owl#ObjectProperty> .
<http://vcell.org/sbpax3#SBState> <http://www.w3.org/2000/01/rdf-schema#comment> "An entity that describes the state of a system. This state can be described by sub elements, whcih makes it usefull to group data that correspond to the same state."^^<http://www.w3.org/2001/XMLSchema#string> .
<http://vcell.org/sbpax3#SBState> <http://www.w3.org/2000/01/rdf-schema#subClassOf> <http://vcell.org/sbpax3#SBEntity> .
<http://vcell.org/sbpax3#SBState> <http://www.w3.org/1999/02/22-rdf-syntax-ns#type> <http://www.w3.org/2002/07/owl#Class> .
<http://vcell.org/sbpax3#hasUnit> <http://www.w3.org/2000/01/rdf-schema#comment> "An instance of uome-core:UnitOfMeasurement representing the unit connected to this measurable systems biology entity.\nExamples: uome-list:Metre, uome-list:Kilogram, uome-list:MicrogramPerMillilitre"^^<http://www.w3.org/2001/XMLSchema#string> .
<http://vcell.org/sbpax3#hasUnit> <http://www.w3.org/2000/01/rdf-schema#range> <http://vcell.org/uome/expressions/#UnitOfMeasurement> .
<http://vcell.org/sbpax3#hasUnit> <http://www.w3.org/2000/01/rdf-schema#domain> <http://vcell.org/sbpax3#SBMeasurable> .
<http://vcell.org/sbpax3#hasUnit> <http://www.w3.org/1999/02/22-rdf-syntax-ns#type> <http://www.w3.org/2002/07/owl#ObjectProperty> .
