@prefix dc: <http://purl.org/dc/elements/1.1/> .
@prefix ex: <http://example.org/> .
@prefix bqbiol: <http://biomodels.net/biology-qualifiers/> .
@prefix foaf: <http://xmlns.com/foaf/0.1/> .
@prefix uome-list: <http://www.sbpax.org/uome/list.owl#> .
@prefix vcard: <http://www.w3.org/2001/vcard-rdf/3.0#> .
@prefix dcterms: <http://purl.org/dc/terms/> .
@prefix rdfs: <http://www.w3.org/2000/01/rdf-schema#> .
@prefix bp3: <http://www.biopax.org/release/biopax-level3.owl#> .
@prefix xmls: <http://www.w3.org/2001/XMLSchema#> .
@prefix bqmodel: <http://biomodels.net/model-qualifiers/> .
@prefix owl: <http://www.w3.org/2002/07/owl#> .
@prefix uome-core: <http://www.sbpax.org/uome/core.owl#> .
@prefix sbx3: <http://vcell.org/sbpax3#> .
@prefix rdf: <http://www.w3.org/1999/02/22-rdf-syntax-ns#> .

<http://vcell.org/sbpax3> a owl:Ontology ;
	owl:imports <http://www.biopax.org/release/biopax-level3.owl> , <http://www.sbpax.org/uome/core.owl> .

sbx3:SBEntity a owl:Class ;
	rdfs:comment """An entity that can be characterized by one or more systems biology terms.
Examples: a BioPAX entity; a rate law or a parameter in a particular instance."""^^xmls:string .

sbx3:SBMeasurable a owl:Class ;
	rdfs:comment """An entity that can be characterized by one or more systems biology terms and that can be represented by a number and a unit.
Example: a parameter in a particular instance."""^^xmls:string ;
	rdfs:subClassOf sbx3:SBEntity .

sbx3:SBState a owl:Class ;
	rdfs:comment "An entity that describes the state of a system. This state can be described by sub elements, whcih makes it usefull to group data that correspond to the same state."^^xmls:string ;
	rdfs:subClassOf sbx3:SBEntity .

sbx3:SBVocabulary a owl:Class ;
	rdfs:comment """Controlled vocabulary that describes a systems biology concept, such as a Systems Biology Ontology term.
Examples: an SBO term; an SBML element name"""^^xmls:string ;
	rdfs:subClassOf bp3:ControlledVocabulary .

sbx3:hasNumber a owl:DatatypeProperty ;
	rdfs:comment """The number representing this measurable systems biology entity.
Example: a concentration of 5 mol/l would have the number 5 together with the unit string \"mol/l\""""^^xmls:string ;
	rdfs:domain sbx3:SBEntity ;
	rdfs:range xmls:float .

sbx3:hasUnit a owl:ObjectProperty ;
	rdfs:comment """An instance of uome-core:UnitOfMeasurement representing the unit connected to this measurable systems biology entity.
Examples: uome-list:Metre, uome-list:Kilogram, uome-list:MicrogramPerMillilitre"""^^xmls:string ;
	rdfs:domain sbx3:SBMeasurable ;
	rdfs:range uome-core:UnitOfMeasurement .

sbx3:sbSubEntity a owl:ObjectProperty ;
	rdfs:comment """A systems biology entity that is a part, attribute or subset of this systems biology entity.
Examples: rate law of an interaction; parameters of a rate law."""^^xmls:string ;
	rdfs:domain sbx3:SBEntity ;
	rdfs:range sbx3:SBEntity .

sbx3:sbTerm a owl:ObjectProperty ;
	rdfs:comment """The systems biology term that this entity is an instance of.
Examples: an SBO term; an SBML element name."""^^xmls:string ;
	rdfs:domain sbx3:SBEntity ;
	rdfs:range sbx3:SBVocabulary .

bp3:Entity rdfs:subClassOf sbx3:SBEntity .
