<http://vcell.org/uome/expressions/#withExponent> <http://www.w3.org/2000/01/rdf-schema#comment> "The exponent in an exponent expression.\nExample: the 2 in m^2."^^<http://www.w3.org/2001/XMLSchema#string> .
<http://vcell.org/uome/expressions/#withExponent> <http://www.w3.org/2000/01/rdf-schema#range> <http://www.w3.org/2001/XMLSchema#double> .
<http://vcell.org/uome/expressions/#withExponent> <http://www.w3.org/2000/01/rdf-schema#domain> <http://vcell.org/uome/expressions/#ExponentialExpression> .
<http://vcell.org/uome/expressions/#withExponent> <http://www.w3.org/1999/02/22-rdf-syntax-ns#type> <http://www.w3.org/2002/07/owl#DatatypeProperty> .
_:A44d577adX3aX13043323d9fX3aXX2dX7f3d <http://www.w3.org/2002/07/owl#minCardinality> "1"^^<http://www.w3.org/2001/XMLSchema#int> .
_:A44d577adX3aX13043323d9fX3aXX2dX7f3d <http://www.w3.org/2002/07/owl#onProperty> <http://vcell.org/uome/expressions/#unitName> .
_:A44d577adX3aX13043323d9fX3aXX2dX7f3d <http://www.w3.org/1999/02/22-rdf-syntax-ns#type> <http://www.w3.org/2002/07/owl#Restriction> .
<http://vcell.org/uome/expressions/#withFactor> <http://www.w3.org/2000/01/rdf-schema#comment> "The factor in a scaling expression.\nExample: the 1000 in 1000*m"^^<http://www.w3.org/2001/XMLSchema#string> .
<http://vcell.org/uome/expressions/#withFactor> <http://www.w3.org/2000/01/rdf-schema#range> <http://www.w3.org/2001/XMLSchema#double> .
<http://vcell.org/uome/expressions/#withFactor> <http://www.w3.org/2000/01/rdf-schema#domain> <http://vcell.org/uome/expressions/#ScalingExpression> .
<http://vcell.org/uome/expressions/#withFactor> <http://www.w3.org/1999/02/22-rdf-syntax-ns#type> <http://www.w3.org/2002/07/owl#DatatypeProperty> .
<http://vcell.org/uome/expressions/#Expression> <http://www.w3.org/2000/01/rdf-schema#comment> "An expression deriving a unit from other units and numbers.\nExample: square meter can be derived by taking meter to the power of two."^^<http://www.w3.org/2001/XMLSchema#string> .
<http://vcell.org/uome/expressions/#Expression> <http://www.w3.org/1999/02/22-rdf-syntax-ns#type> <http://www.w3.org/2002/07/owl#Class> .
<http://vcell.org/uome/expressions/#EquivalenzExpression> <http://www.w3.org/2000/01/rdf-schema#comment> "An expression deriving a unit by declaring it equivalent to another.\nExample: radian is equivalent to the dimensionless unit."^^<http://www.w3.org/2001/XMLSchema#string> .
<http://vcell.org/uome/expressions/#EquivalenzExpression> <http://www.w3.org/2000/01/rdf-schema#subClassOf> <http://vcell.org/uome/expressions/#SingleUnitExpression> .
<http://vcell.org/uome/expressions/#EquivalenzExpression> <http://www.w3.org/1999/02/22-rdf-syntax-ns#type> <http://www.w3.org/2002/07/owl#Class> .
<http://vcell.org/uome/expressions/#ScalingExpression> <http://www.w3.org/2000/01/rdf-schema#comment> "An expression deriving a unit by scaling an original unit with a number.\nExample: microns can be derived from meter scaled by 1e-3."^^<http://www.w3.org/2001/XMLSchema#string> .
<http://vcell.org/uome/expressions/#ScalingExpression> <http://www.w3.org/2000/01/rdf-schema#subClassOf> _:A44d577adX3aX13043323d9fX3aXX2dX7f3a .
<http://vcell.org/uome/expressions/#ScalingExpression> <http://www.w3.org/2000/01/rdf-schema#subClassOf> <http://vcell.org/uome/expressions/#SingleUnitExpression> .
<http://vcell.org/uome/expressions/#ScalingExpression> <http://www.w3.org/1999/02/22-rdf-syntax-ns#type> <http://www.w3.org/2002/07/owl#Class> .
_:A44d577adX3aX13043323d9fX3aXX2dX7f39 <http://www.w3.org/2002/07/owl#cardinality> "1"^^<http://www.w3.org/2001/XMLSchema#int> .
_:A44d577adX3aX13043323d9fX3aXX2dX7f39 <http://www.w3.org/2002/07/owl#onProperty> <http://vcell.org/uome/expressions/#withOffset> .
_:A44d577adX3aX13043323d9fX3aXX2dX7f39 <http://www.w3.org/1999/02/22-rdf-syntax-ns#type> <http://www.w3.org/2002/07/owl#Restriction> .
<http://vcell.org/uome/expressions/#UnitOfMeasurementVocabulary> <http://www.w3.org/2000/01/rdf-schema#comment> "Vocabulary to describe a unit of measurement.\nExample: a term form the Unit Ontology."^^<http://www.w3.org/2001/XMLSchema#string> .
<http://vcell.org/uome/expressions/#UnitOfMeasurementVocabulary> <http://www.w3.org/2000/01/rdf-schema#subClassOf> <http://www.biopax.org/release/biopax-level3.owl#ControlledVocabulary> .
<http://vcell.org/uome/expressions/#UnitOfMeasurementVocabulary> <http://www.w3.org/1999/02/22-rdf-syntax-ns#type> <http://www.w3.org/2002/07/owl#Class> .
<http://vcell.org/uome/expressions/#unitSymbol> <http://www.w3.org/2000/01/rdf-schema#comment> "The symbol of a unit.\nExamples: m, K, min."^^<http://www.w3.org/2001/XMLSchema#string> .
<http://vcell.org/uome/expressions/#unitSymbol> <http://www.w3.org/2000/01/rdf-schema#range> <http://www.w3.org/2001/XMLSchema#string> .
<http://vcell.org/uome/expressions/#unitSymbol> <http://www.w3.org/2000/01/rdf-schema#domain> <http://vcell.org/uome/expressions/#UnitOfMeasurement> .
<http://vcell.org/uome/expressions/#unitSymbol> <http://www.w3.org/1999/02/22-rdf-syntax-ns#type> <http://www.w3.org/2002/07/owl#DatatypeProperty> .
_:A44d577adX3aX13043323d9fX3aXX2dX7f3c <http://www.w3.org/2002/07/owl#minCardinality> "1"^^<http://www.w3.org/2001/XMLSchema#int> .
_:A44d577adX3aX13043323d9fX3aXX2dX7f3c <http://www.w3.org/2002/07/owl#onProperty> <http://vcell.org/uome/expressions/#unitSymbol> .
_:A44d577adX3aX13043323d9fX3aXX2dX7f3c <http://www.w3.org/1999/02/22-rdf-syntax-ns#type> <http://www.w3.org/2002/07/owl#Restriction> .
<http://vcell.org/uome/expressions/#derivedBy> <http://www.w3.org/2000/01/rdf-schema#comment> "An expression that can be used to derive this unit.\nExample: J can be derived by the product N*m."^^<http://www.w3.org/2001/XMLSchema#string> .
<http://vcell.org/uome/expressions/#derivedBy> <http://www.w3.org/1999/02/22-rdf-syntax-ns#type> <http://www.w3.org/2002/07/owl#ObjectProperty> .
_:A44d577adX3aX13043323d9fX3aXX2dX7f38 <http://www.w3.org/2002/07/owl#cardinality> "1"^^<http://www.w3.org/2001/XMLSchema#int> .
_:A44d577adX3aX13043323d9fX3aXX2dX7f38 <http://www.w3.org/2002/07/owl#onProperty> <http://vcell.org/uome/expressions/#withExponent> .
_:A44d577adX3aX13043323d9fX3aXX2dX7f38 <http://www.w3.org/1999/02/22-rdf-syntax-ns#type> <http://www.w3.org/2002/07/owl#Restriction> .
_:A44d577adX3aX13043323d9fX3aXX2dX7f37 <http://www.w3.org/2002/07/owl#cardinality> "1"^^<http://www.w3.org/2001/XMLSchema#int> .
_:A44d577adX3aX13043323d9fX3aXX2dX7f37 <http://www.w3.org/2002/07/owl#onProperty> <http://vcell.org/uome/expressions/#withUnit1> .
_:A44d577adX3aX13043323d9fX3aXX2dX7f37 <http://www.w3.org/1999/02/22-rdf-syntax-ns#type> <http://www.w3.org/2002/07/owl#Restriction> .
_:A44d577adX3aX13043323d9fX3aXX2dX7f3b <http://www.w3.org/2002/07/owl#cardinality> "1"^^<http://www.w3.org/2001/XMLSchema#int> .
_:A44d577adX3aX13043323d9fX3aXX2dX7f3b <http://www.w3.org/2002/07/owl#onProperty> <http://vcell.org/uome/expressions/#withUnit> .
_:A44d577adX3aX13043323d9fX3aXX2dX7f3b <http://www.w3.org/1999/02/22-rdf-syntax-ns#type> <http://www.w3.org/2002/07/owl#Restriction> .
<http://vcell.org/uome/expressions/#withUnit2> <http://www.w3.org/2000/01/rdf-schema#comment> "The second unit in a binary expression of units.\nExample: the s in m/s"^^<http://www.w3.org/2001/XMLSchema#string> .
<http://vcell.org/uome/expressions/#withUnit2> <http://www.w3.org/2000/01/rdf-schema#range> <http://vcell.org/uome/expressions/#UnitOfMeasurement> .
<http://vcell.org/uome/expressions/#withUnit2> <http://www.w3.org/2000/01/rdf-schema#domain> <http://vcell.org/uome/expressions/#BinaryExpression> .
<http://vcell.org/uome/expressions/#withUnit2> <http://www.w3.org/1999/02/22-rdf-syntax-ns#type> <http://www.w3.org/2002/07/owl#ObjectProperty> .
<http://vcell.org/uome/expressions/#OffsetExpression> <http://www.w3.org/2000/01/rdf-schema#comment> "An expression deriving a unit offsetting the zero-point of an original unit by a number.\nExample: celsius can be derived from kelvin by offsetting the zero-point by about 273."^^<http://www.w3.org/2001/XMLSchema#string> .
<http://vcell.org/uome/expressions/#OffsetExpression> <http://www.w3.org/2000/01/rdf-schema#subClassOf> _:A44d577adX3aX13043323d9fX3aXX2dX7f39 .
<http://vcell.org/uome/expressions/#OffsetExpression> <http://www.w3.org/2000/01/rdf-schema#subClassOf> <http://vcell.org/uome/expressions/#Expression> .
<http://vcell.org/uome/expressions/#OffsetExpression> <http://www.w3.org/1999/02/22-rdf-syntax-ns#type> <http://www.w3.org/2002/07/owl#Class> .
<http://vcell.org/uome/expressions/#unitTerm> <http://www.w3.org/2000/01/rdf-schema#comment> "The controlled vocabulary term describing a unit.\nExamples: m, K, min."^^<http://www.w3.org/2001/XMLSchema#string> .
<http://vcell.org/uome/expressions/#unitTerm> <http://www.w3.org/2000/01/rdf-schema#range> <http://vcell.org/uome/expressions/#UnitOfMeasurementVocabulary> .
<http://vcell.org/uome/expressions/#unitTerm> <http://www.w3.org/2000/01/rdf-schema#domain> <http://vcell.org/uome/expressions/#UnitOfMeasurement> .
<http://vcell.org/uome/expressions/#unitTerm> <http://www.w3.org/1999/02/22-rdf-syntax-ns#type> <http://www.w3.org/2002/07/owl#ObjectProperty> .
<http://vcell.org/uome/expressions/#UnitOfMeasurement> <http://www.w3.org/2000/01/rdf-schema#comment> "A unit used to describe anything measurable in the widest sense. Includes anything definitely quantifiable.\nExample: kilogram, litre, ampere, minute, inch, fluid ounce, psi."^^<http://www.w3.org/2001/XMLSchema#string> .
<http://vcell.org/uome/expressions/#UnitOfMeasurement> <http://www.w3.org/2000/01/rdf-schema#subClassOf> _:A44d577adX3aX13043323d9fX3aXX2dX7f3c .
<http://vcell.org/uome/expressions/#UnitOfMeasurement> <http://www.w3.org/2000/01/rdf-schema#subClassOf> _:A44d577adX3aX13043323d9fX3aXX2dX7f3d .
<http://vcell.org/uome/expressions/#UnitOfMeasurement> <http://www.w3.org/1999/02/22-rdf-syntax-ns#type> <http://www.w3.org/2002/07/owl#Class> .
<http://vcell.org/uome/expressions/#BinaryExpression> <http://www.w3.org/2000/01/rdf-schema#comment> "An expression deriving a unit involving two other units\nExamples: product or quotient of units."^^<http://www.w3.org/2001/XMLSchema#string> .
<http://vcell.org/uome/expressions/#BinaryExpression> <http://www.w3.org/2000/01/rdf-schema#subClassOf> _:A44d577adX3aX13043323d9fX3aXX2dX7f36 .
<http://vcell.org/uome/expressions/#BinaryExpression> <http://www.w3.org/2000/01/rdf-schema#subClassOf> _:A44d577adX3aX13043323d9fX3aXX2dX7f37 .
<http://vcell.org/uome/expressions/#BinaryExpression> <http://www.w3.org/2000/01/rdf-schema#subClassOf> <http://vcell.org/uome/expressions/#Expression> .
<http://vcell.org/uome/expressions/#BinaryExpression> <http://www.w3.org/1999/02/22-rdf-syntax-ns#type> <http://www.w3.org/2002/07/owl#Class> .
<http://vcell.org/uome/expressions/#withUnit> <http://www.w3.org/2000/01/rdf-schema#comment> "The unit in an expression that contains only one unit.\nExample: the m in 1000*m"^^<http://www.w3.org/2001/XMLSchema#string> .
<http://vcell.org/uome/expressions/#withUnit> <http://www.w3.org/2000/01/rdf-schema#range> <http://vcell.org/uome/expressions/#UnitOfMeasurement> .
<http://vcell.org/uome/expressions/#withUnit> <http://www.w3.org/2000/01/rdf-schema#domain> <http://vcell.org/uome/expressions/#SingleUnitExpression> .
<http://vcell.org/uome/expressions/#withUnit> <http://www.w3.org/1999/02/22-rdf-syntax-ns#type> <http://www.w3.org/2002/07/owl#ObjectProperty> .
<http://vcell.org/uome/expressions/#ProductExpression> <http://www.w3.org/2000/01/rdf-schema#comment> "An expression deriving a unit by multiplying two other units\nExamples: joule can be derived as the product of newton and metre."^^<http://www.w3.org/2001/XMLSchema#string> .
<http://vcell.org/uome/expressions/#ProductExpression> <http://www.w3.org/2000/01/rdf-schema#subClassOf> <http://vcell.org/uome/expressions/#BinaryExpression> .
<http://vcell.org/uome/expressions/#ProductExpression> <http://www.w3.org/1999/02/22-rdf-syntax-ns#type> <http://www.w3.org/2002/07/owl#Class> .
<http://vcell.org/uome/expressions/#SingleUnitExpression> <http://www.w3.org/2000/01/rdf-schema#comment> "An expression deriving a unit involving one other unit.\nExamples: multiplication, exponentiation and offset of a unit by a number."^^<http://www.w3.org/2001/XMLSchema#string> .
<http://vcell.org/uome/expressions/#SingleUnitExpression> <http://www.w3.org/2000/01/rdf-schema#subClassOf> _:A44d577adX3aX13043323d9fX3aXX2dX7f3b .
<http://vcell.org/uome/expressions/#SingleUnitExpression> <http://www.w3.org/2000/01/rdf-schema#subClassOf> <http://vcell.org/uome/expressions/#Expression> .
<http://vcell.org/uome/expressions/#SingleUnitExpression> <http://www.w3.org/1999/02/22-rdf-syntax-ns#type> <http://www.w3.org/2002/07/owl#Class> .
_:A44d577adX3aX13043323d9fX3aXX2dX7f3a <http://www.w3.org/2002/07/owl#cardinality> "1"^^<http://www.w3.org/2001/XMLSchema#int> .
_:A44d577adX3aX13043323d9fX3aXX2dX7f3a <http://www.w3.org/2002/07/owl#onProperty> <http://vcell.org/uome/expressions/#withFactor> .
_:A44d577adX3aX13043323d9fX3aXX2dX7f3a <http://www.w3.org/1999/02/22-rdf-syntax-ns#type> <http://www.w3.org/2002/07/owl#Restriction> .
<http://vcell.org/uome/expressions/#withUnit1> <http://www.w3.org/2000/01/rdf-schema#comment> "The first unit in a binary expression of units.\nExample: the m in m/s"^^<http://www.w3.org/2001/XMLSchema#string> .
<http://vcell.org/uome/expressions/#withUnit1> <http://www.w3.org/2000/01/rdf-schema#range> <http://vcell.org/uome/expressions/#UnitOfMeasurement> .
<http://vcell.org/uome/expressions/#withUnit1> <http://www.w3.org/2000/01/rdf-schema#domain> <http://vcell.org/uome/expressions/#BinaryExpression> .
<http://vcell.org/uome/expressions/#withUnit1> <http://www.w3.org/1999/02/22-rdf-syntax-ns#type> <http://www.w3.org/2002/07/owl#ObjectProperty> .
<http://vcell.org/uome/expressions/#QuotientExpression> <http://www.w3.org/2000/01/rdf-schema#comment> "An expression deriving a unit from two other units by dividing one of those by the other.\nExamples: watt can be derived as the quotient of joule and second."^^<http://www.w3.org/2001/XMLSchema#string> .
<http://vcell.org/uome/expressions/#QuotientExpression> <http://www.w3.org/2000/01/rdf-schema#subClassOf> <http://vcell.org/uome/expressions/#BinaryExpression> .
<http://vcell.org/uome/expressions/#QuotientExpression> <http://www.w3.org/1999/02/22-rdf-syntax-ns#type> <http://www.w3.org/2002/07/owl#Class> .
_:A44d577adX3aX13043323d9fX3aXX2dX7f36 <http://www.w3.org/2002/07/owl#cardinality> "1"^^<http://www.w3.org/2001/XMLSchema#int> .
_:A44d577adX3aX13043323d9fX3aXX2dX7f36 <http://www.w3.org/2002/07/owl#onProperty> <http://vcell.org/uome/expressions/#withUnit2> .
_:A44d577adX3aX13043323d9fX3aXX2dX7f36 <http://www.w3.org/1999/02/22-rdf-syntax-ns#type> <http://www.w3.org/2002/07/owl#Restriction> .
<http://vcell.org/uome/expressions/#withOffset> <http://www.w3.org/2000/01/rdf-schema#comment> "The zero-point of the expressed units in terms of the original unit.\nExample: to get an expression for celsius, create an offset expression with unit Kelvin and an offset of about 273, because the zero-point of celsius is at about 273 kelvin"^^<http://www.w3.org/2001/XMLSchema#string> .
<http://vcell.org/uome/expressions/#withOffset> <http://www.w3.org/2000/01/rdf-schema#range> <http://www.w3.org/2001/XMLSchema#double> .
<http://vcell.org/uome/expressions/#withOffset> <http://www.w3.org/2000/01/rdf-schema#domain> <http://vcell.org/uome/expressions/#OffsetExpression> .
<http://vcell.org/uome/expressions/#withOffset> <http://www.w3.org/1999/02/22-rdf-syntax-ns#type> <http://www.w3.org/2002/07/owl#DatatypeProperty> .
<http://vcell.org/uome/expressions/#unitName> <http://www.w3.org/2000/01/rdf-schema#comment> "The name of a unit.\nExamples: meter, kelvin, minute."^^<http://www.w3.org/2001/XMLSchema#string> .
<http://vcell.org/uome/expressions/#unitName> <http://www.w3.org/2000/01/rdf-schema#range> <http://www.w3.org/2001/XMLSchema#string> .
<http://vcell.org/uome/expressions/#unitName> <http://www.w3.org/2000/01/rdf-schema#domain> <http://vcell.org/uome/expressions/#UnitOfMeasurement> .
<http://vcell.org/uome/expressions/#unitName> <http://www.w3.org/1999/02/22-rdf-syntax-ns#type> <http://www.w3.org/2002/07/owl#DatatypeProperty> .
<http://vcell.org/uome/expressions/#ExponentialExpression> <http://www.w3.org/2000/01/rdf-schema#comment> "An expression deriving a unit by exponentiating an original unit by a number.\nExample: square meter can be derived by taking meter to the power of two."^^<http://www.w3.org/2001/XMLSchema#string> .
<http://vcell.org/uome/expressions/#ExponentialExpression> <http://www.w3.org/2000/01/rdf-schema#subClassOf> _:A44d577adX3aX13043323d9fX3aXX2dX7f38 .
<http://vcell.org/uome/expressions/#ExponentialExpression> <http://www.w3.org/2000/01/rdf-schema#subClassOf> <http://vcell.org/uome/expressions/#Expression> .
<http://vcell.org/uome/expressions/#ExponentialExpression> <http://www.w3.org/1999/02/22-rdf-syntax-ns#type> <http://www.w3.org/2002/07/owl#Class> .
<http://vcell.org/uome/expressions/> <http://www.w3.org/2002/07/owl#imports> <http://www.biopax.org/release/biopax-level3.owl> .
<http://vcell.org/uome/expressions/> <http://www.w3.org/1999/02/22-rdf-syntax-ns#type> <http://www.w3.org/2002/07/owl#Ontology> .
