@prefix dc: <http://purl.org/dc/elements/1.1/> .
@prefix ex: <http://example.org/> .
@prefix bqbiol: <http://biomodels.net/biology-qualifiers/> .
@prefix foaf: <http://xmlns.com/foaf/0.1/> .
@prefix uome-list: <http://www.sbpax.org/uome/list.owl#> .
@prefix vcard: <http://www.w3.org/2001/vcard-rdf/3.0#> .
@prefix dcterms: <http://purl.org/dc/terms/> .
@prefix rdfs: <http://www.w3.org/2000/01/rdf-schema#> .
@prefix bp3: <http://www.biopax.org/release/biopax-level3.owl#> .
@prefix xmls: <http://www.w3.org/2001/XMLSchema#> .
@prefix bqmodel: <http://biomodels.net/model-qualifiers/> .
@prefix owl: <http://www.w3.org/2002/07/owl#> .
@prefix uome-core: <http://www.sbpax.org/uome/core.owl#> .
@prefix sbx3: <http://vcell.org/sbpax3#> .
@prefix rdf: <http://www.w3.org/1999/02/22-rdf-syntax-ns#> .

<http://www.sbpax.org/uome/core.owl> a owl:Ontology ;
	owl:imports <http://www.biopax.org/release/biopax-level3.owl> .

uome-core:BinaryExpression a owl:Class ;
	rdfs:comment """An expression deriving a unit involving two other units
Examples: product or quotient of units."""^^xmls:string ;
	rdfs:subClassOf uome-core:Expression , _:node16dgehbd3x199 , _:node16dgehbd3x200 .

uome-core:EquivalenzExpression a owl:Class ;
	rdfs:comment """An expression deriving a unit by declaring it equivalent to another.
Example: radian is equivalent to the dimensionless unit."""^^xmls:string ;
	rdfs:subClassOf uome-core:SingleUnitExpression .

uome-core:ExponentialExpression a owl:Class ;
	rdfs:comment """An expression deriving a unit by exponentiating an original unit by a number.
Example: square meter can be derived by taking meter to the power of two."""^^xmls:string ;
	rdfs:subClassOf uome-core:SingleUnitExpression , _:node16dgehbd3x198 .

uome-core:Expression a owl:Class ;
	rdfs:comment """An expression deriving a unit from other units and numbers.
Example: square meter can be derived by taking meter to the power of two."""^^xmls:string .

uome-core:OffsetExpression a owl:Class ;
	rdfs:comment """An expression deriving a unit offsetting the zero-point of an original unit by a number.
Example: celsius can be derived from kelvin by offsetting the zero-point by about 273."""^^xmls:string ;
	rdfs:subClassOf uome-core:SingleUnitExpression , _:node16dgehbd3x197 .

uome-core:ProductExpression a owl:Class ;
	rdfs:comment """An expression deriving a unit by multiplying two other units
Examples: joule can be derived as the product of newton and metre."""^^xmls:string ;
	rdfs:subClassOf uome-core:BinaryExpression .

uome-core:QuotientExpression a owl:Class ;
	rdfs:comment """An expression deriving a unit from two other units by dividing one of those by the other.
Examples: watt can be derived as the quotient of joule and second."""^^xmls:string ;
	rdfs:subClassOf uome-core:BinaryExpression .

uome-core:ScalingExpression a owl:Class ;
	rdfs:comment """An expression deriving a unit by scaling an original unit with a number.
Example: microns can be derived from meter scaled by 1e-3."""^^xmls:string ;
	rdfs:subClassOf uome-core:SingleUnitExpression , _:node16dgehbd3x196 .

uome-core:SingleUnitExpression a owl:Class ;
	rdfs:comment """An expression deriving a unit involving one other unit.
Examples: multiplication, exponentiation and offset of a unit by a number."""^^xmls:string ;
	rdfs:subClassOf uome-core:Expression , _:node16dgehbd3x195 .

uome-core:UnitOfMeasurement a owl:Class ;
	rdfs:comment """A unit used to describe anything measurable in the widest sense. Includes anything definitely quantifiable.
Example: kilogram, litre, ampere, minute, inch, fluid ounce, psi."""^^xmls:string ;
	rdfs:subClassOf _:node16dgehbd3x193 , _:node16dgehbd3x194 .

uome-core:UnitOfMeasurementVocabulary a owl:Class ;
	rdfs:comment """Vocabulary to describe a unit of measurement.
Example: a term form the Unit Ontology."""^^xmls:string ;
	rdfs:subClassOf bp3:ControlledVocabulary .

uome-core:derivedBy a owl:ObjectProperty ;
	rdfs:comment """An expression that can be used to derive this unit.
Example: J can be derived by the product N*m."""^^xmls:string .

uome-core:unitName a owl:DatatypeProperty ;
	rdfs:comment """The name of a unit.
Examples: meter, kelvin, minute."""^^xmls:string ;
	rdfs:domain uome-core:UnitOfMeasurement ;
	rdfs:range xmls:string .

uome-core:unitSymbol a owl:DatatypeProperty ;
	rdfs:comment """The symbol of a unit.
Examples: m, K, min."""^^xmls:string ;
	rdfs:domain uome-core:UnitOfMeasurement ;
	rdfs:range xmls:string .

uome-core:unitTerm a owl:ObjectProperty ;
	rdfs:comment """The controlled vocabulary term describing a unit.
Examples: m, K, min."""^^xmls:string ;
	rdfs:domain uome-core:UnitOfMeasurement ;
	rdfs:range uome-core:UnitOfMeasurementVocabulary .

uome-core:withExponent a owl:DatatypeProperty ;
	rdfs:comment """The exponent in an exponent expression.
Example: the 2 in m^2."""^^xmls:string ;
	rdfs:domain uome-core:ExponentialExpression ;
	rdfs:range xmls:string .

uome-core:withFactor a owl:DatatypeProperty ;
	rdfs:comment """The factor in a scaling expression.
Example: the 1000 in 1000*m"""^^xmls:string ;
	rdfs:domain uome-core:ScalingExpression ;
	rdfs:range xmls:double .

uome-core:withOffset a owl:DatatypeProperty ;
	rdfs:comment """The zero-point of the expressed units in terms of the original unit.
Example: to get an expression for celsius, create an offset expression with unit Kelvin and an offset of about 273, because the zero-point of celsius is at about 273 kelvin"""^^xmls:string ;
	rdfs:domain uome-core:OffsetExpression ;
	rdfs:range xmls:double .

uome-core:withUnit a owl:ObjectProperty ;
	rdfs:comment """The unit in an expression that contains only one unit.
Example: the m in 1000*m"""^^xmls:string ;
	rdfs:domain uome-core:SingleUnitExpression ;
	rdfs:range uome-core:UnitOfMeasurement .

uome-core:withUnit1 a owl:ObjectProperty ;
	rdfs:comment """The first unit in a binary expression of units.
Example: the m in m/s"""^^xmls:string ;
	rdfs:domain uome-core:BinaryExpression ;
	rdfs:range uome-core:UnitOfMeasurement .

uome-core:withUnit2 a owl:ObjectProperty ;
	rdfs:comment """The second unit in a binary expression of units.
Example: the s in m/s"""^^xmls:string ;
	rdfs:domain uome-core:BinaryExpression ;
	rdfs:range uome-core:UnitOfMeasurement .

_:node16dgehbd3x193 a owl:Restriction ;
	owl:minCardinality "1"^^xmls:int ;
	owl:onProperty uome-core:unitName .

_:node16dgehbd3x194 a owl:Restriction ;
	owl:minCardinality "1"^^xmls:int ;
	owl:onProperty uome-core:unitSymbol .

_:node16dgehbd3x195 a owl:Restriction ;
	owl:cardinality "1"^^xmls:int ;
	owl:onProperty uome-core:withUnit .

_:node16dgehbd3x196 a owl:Restriction ;
	owl:cardinality "1"^^xmls:int ;
	owl:onProperty uome-core:withFactor .

_:node16dgehbd3x197 a owl:Restriction ;
	owl:cardinality "1"^^xmls:int ;
	owl:onProperty uome-core:withOffset .

_:node16dgehbd3x198 a owl:Restriction ;
	owl:cardinality "1"^^xmls:int ;
	owl:onProperty uome-core:withExponent .

_:node16dgehbd3x199 a owl:Restriction ;
	owl:cardinality "1"^^xmls:int ;
	owl:onProperty uome-core:withUnit1 .

_:node16dgehbd3x200 a owl:Restriction ;
	owl:cardinality "1"^^xmls:int ;
	owl:onProperty uome-core:withUnit2 .
